Review edits

docs/HowToFAQ/FAQFunctionUnroll1.dfy
@@ -1,27 +1,27 @@
-function {:fuel 10} LengthSum(s: seq<string>): nat {
+function {:fuel 10} Sum(s: seq<string>): nat {
   if |s| == 0 then 0
-  else |s[0]| + LengthSum(s[1..])
+  else |s[0]| + Sum(s[1..])
 }
 
-lemma LengthSum1(s: seq<string>)
+lemma Sum1(s: seq<string>)
   requires |s| == 1
-  ensures LengthSum(s) == |s[0]|
+  ensures Sum(s) == |s[0]|
 {
   // trivial
 }
 
-lemma LengthSum2(s: seq<string>)
+lemma Sum2(s: seq<string>)
   requires |s| == 2
-  ensures LengthSum(s) == |s[0]| + |s[1]|
+  ensures Sum(s) == |s[0]| + |s[1]|
 {
   // Doesn't work.  I need...
-  // LengthSum1(s[1..]);
+  // Sum1(s[1..]);
 }
 
-lemma LengthSum3(s: seq<string>)
+lemma Sum3(s: seq<string>)
   requires |s| == 3
-  ensures LengthSum(s) == |s[0]| + |s[1]| + |s[2]|
+  ensures Sum(s) == |s[0]| + |s[1]| + |s[2]|
 {
   // Doesn't work.  I need...
-  // LengthSum2(s[1..]);
+  // Sum2(s[1..]);
 }
