docs/HowToFAQ/FAQFunctionUnroll2.dfy
@@ -1,33 +1,33 @@
-function LengthSum(s: seq<string>): nat {
+function Sum(s: seq<string>): nat {
   if |s| == 0 then 0
-  else |s[0]| + LengthSum(s[1..])
+  else |s[0]| + Sum(s[1..])
 }
 
-function LengthSum_(s: seq<string>, n: nat): nat
-  ensures LengthSum(s) == LengthSum_(s,n)
-  ensures |s| > 0 && n > 0 ==> LengthSum_(s,n) == |s[0]| + LengthSum_(s[1..], n-1)
+function Sum_(s: seq<string>, n: nat): nat
+  ensures Sum(s) == Sum_(s,n)
+  ensures |s| > 0 && n > 0 ==> Sum_(s,n) == |s[0]| + Sum_(s[1..], n-1)
 {
-  if |s| == 0 || n == 0 then LengthSum(s)
-              else |s[0]| + LengthSum_(s[1..], n-1)
+  if |s| == 0 || n == 0 then Sum(s)
+  else |s[0]| + Sum_(s[1..], n-1)
 }
 
-lemma LengthSum1(s: seq<string>)
+lemma Sum1(s: seq<string>)
   requires |s| == 1
-  ensures LengthSum(s) == |s[0]|
+  ensures Sum(s) == |s[0]|
 {
   // trivial
 }
 
-lemma LengthSum3(s: seq<string>)
+lemma Sum3(s: seq<string>)
   requires |s| == 3
-  ensures LengthSum(s) == |s[0]| + |s[1]| + |s[2]|
+  ensures Sum(s) == |s[0]| + |s[1]| + |s[2]|
 {
-  var _ := LengthSum_(s, 3);
+  var _ := Sum_(s, 3);
 }
 
-lemma LengthSum9(s: seq<string>)
+lemma Sum9(s: seq<string>)
   requires |s| == 9
-  ensures LengthSum(s) == |s[0]| + |s[1]| + |s[2]| + |s[3]| + |s[4]| + |s[5]| + |s[6]| + |s[7]| + |s[8]| 
+  ensures Sum(s) == |s[0]| + |s[1]| + |s[2]| + |s[3]| + |s[4]| + |s[5]| + |s[6]| + |s[7]| + |s[8]| 
 {
-  var _ := LengthSum_(s, 9);
+  var _ := Sum_(s, 9);
 }
