docs/HowToFAQ/FAQFunctionUnroll.md
@@ -15,22 +15,24 @@ How can I get this to prove automatically?
 
 ## Answer
 
-Function bodies are transparent. That is, when there is a call to a function in Dafny code, Dafny will insert inline
-the definition of the function. But for recursive functions, it generally only does this once, as just once is 
+Function bodies are transparent. That is, when there is a call to a function in Dafny code, the body of the function
+is available for reasoning about the effect of the function. But for recursive functions, it generally only does this once or twice, as that is 
 usually sufficient to form an inductive proof. And always unrolling multiple times can reduce performance.
 
-You can request that Dafny unroll a function multiple times by using the (unintuitively named) `{:fuel}` attribute.
+You can request that Dafny unroll a function multiple times by using the `{:fuel}` attribute.
 The value of the attribute is the number of times the function will be unrolled. This is still a fixed upper limit,
 but it does the trick in this case:
 ```
 {% include_relative FAQFunctionUnroll1.dfy %}
 ```
 
-A function will also keep unrolling if it has an argument that is a literal `nat` and that argument decreases
+A function will also keep unrolling if it has an argument that is a literal and that argument decreases
 on each recursive call. So for this example we can write a helper function that takes a `nat` argument
 and give it a literal value that tells it how often to unroll.
 ```
 {% include_relative FAQFunctionUnroll2.dfy %}
 ```
 With this solution, the number of unrollings can be set at the call site, rather than in the function definition.
+
+[This paper](https://www.microsoft.com/en-us/research/publication/computing-smt-solver/) gives some technical insight into how recursive functions are handled in situations liek these examples.
 
