docs/HowToFAQ/FAQMultClauses.md
@@ -12,7 +12,7 @@ Multiple ensures clauses, such as `ensures P ensures Q ensures R` is equivalent 
 The order is important if an earlier predicate is needed to be sure that a later one is well defined. For example the two predicates in `ensures a != null ensures a.Length > 0`
 must be in that order because `a.Length` is well-defined only if `a != null`.
 
-In addition, sometimes one ensures clause serves as a lemma for the next one. Without the earlier clause, Dafny can have trouble proving the second one, even though it is valid.
+In addition, sometimes one ensures clause serves as a intermediate reasoning step for the next one. Without the earlier clause, Dafny can have trouble proving the second one, even though it is valid.
 With the first predicate as an intermediate step, the second is then more easily proved.
 
 This order dependence of postconditions is also the case for preconditions and loop invariants
