docs/HowToFAQ/index.md
@@ -24,13 +24,13 @@ If you have questions that are not addressed here, be sure to communicate them t
 - ["Is there a simple way to prove the termination of a recursive function?"](FAQRecursiveTermination)
 
 - ["How do I make a singleton instance of a class for repeated later use?](FAQSingleton)
-- ["Is there a way to write `if foo().equals(bar()) { x } else { y }` where `foo` and `bar` are methods?](FAQMethodSequence)
+- ["Is there a way to use methods within expressions?"](FAQMethodSequence)
 - ["If I have an assertion about a class and a loop that doesn't mention (read, modify)  the class, why does dafny fail to establish the assertion after the loop?"](FAQLoopModifies)
-- ["I can assert a condition right before a return, so why does the postcondition fail?](FAQFailingPost)
+- ["I can assert a condition right before a return, so why does the postcondition fail to verify?](FAQFailingPost)
 - ["How can I combine sequences of different types?"](FAQSeqTrait)
 - ["How do I disambiguate module names?](FAQModuleNames)
 - ["A function seems to work just once. How do I get it to apply a bunch of times?"](FAQFunctionUnroll)
-- ["Why is my import opened statement not working?"](FAQModuleImport)
+- ["Why do nested modules not see the imports of their enclosing modules?"](FAQModuleImport)
 - ["Is there a way to test that two types are the same?"](FAQTypeCompare)
 - ["When a lemma has multiple ensures clauses, I’m finding that they interact, when I expected them to be independent.  For example, commenting out one of them can make another one not verify.  How should I think about this?"](FAQMultClauses)
 
